first attempt at V_of

Q0_Metatheory/Completeness.thy
@@ -2,15 +2,65 @@ theory Completeness imports
     Consistency
 begin
 
+
+instance type :: countable
+  by countable_datatype
+
+instance form :: countable
+  by countable_datatype
+
+instance type :: small ..
+instance type :: embeddable ..
+instance form :: small ..
+instance form :: embeddable ..
+
+definition V_of_type :: "type \<Rightarrow> V" where
+  "V_of_type = (SOME V_of. inj V_of)"
+
+definition type_of_V :: "V \<Rightarrow> type" where
+  "type_of_V = inv V_of_type"
+
+definition is_type :: "V \<Rightarrow> bool" where
+  "is_type t \<longleftrightarrow> t \<in> range V_of_type"
+
+lemma "is_type VA \<Longrightarrow> \<exists>t. V_of_type t = VA "
+  using is_type_def by auto
+
+lemma "inj V_of_type"
+  by (metis V_of_type_def embeddable_class.ex_inj someI_ex)
+  
+lemma "type_of_V (V_of_type t) = t"
+  by (metis V_of_type_def embeddable_class.ex_inj type_of_V_def inv_f_f someI_ex)
+
+lemma "is_type Vt \<Longrightarrow> V_of_type (type_of_V Vt) = Vt"
+  by (simp add: f_inv_into_f is_type_def type_of_V_def)
+
+
+definition V_of_form :: "form \<Rightarrow> V" where
+  "V_of_form = (SOME V_of. inj V_of)"
+
+definition form_of_V :: "V \<Rightarrow> form" where
+  "form_of_V = inv V_of_form"
+
+definition is_form :: "V \<Rightarrow> bool" where
+  "is_form A \<longleftrightarrow> A \<in> range V_of_form"
+
+lemma "is_form VA \<Longrightarrow> \<exists>A. V_of_form A = VA "
+  using is_form_def by auto
+
+lemma "inj V_of_form"
+  by (metis V_of_form_def embeddable_class.ex_inj someI_ex)
+  
+lemma "form_of_V (V_of_form A) = A"
+  by (metis V_of_form_def embeddable_class.ex_inj form_of_V_def inv_f_f someI_ex)
+
+lemma "is_form VA \<Longrightarrow> V_of_form (form_of_V VA) = VA"
+  by (simp add: f_inv_into_f form_of_V_def is_form_def)
+
+
 context
   fixes H :: "form set"
 begin
-
-definition V_of_form :: "form \<Rightarrow> V" where
-  "V_of_form A = undefined A"
-
-definition form_of_V :: "V \<Rightarrow> form" where
-  "form_of_V S = undefined S"
 
 definition V_of_form_set :: "form set \<Rightarrow> V" where
   "V_of_form_set As = set (V_of_form ` As)"
